Q1

From **Theorem 1.7**, we know that
$$
P(B^*(t) \geq a, B(t) \leq x) = 1 - N(\frac{2a - x}{\sqrt{t}}).
$$
Then the cumulative distribution function of $(B(t), B^*(t))$ is
$$
F(x, a) = P(B(t) \leq x, B^*(t) \leq a) = N(\frac{2a - x}{\sqrt{t}}).
$$
So the joint density of $(B(t), B^*(t))$ is 
$$
f(x, a) = \frac{\partial^2 F}{\partial x \partial a} =
$$


Q2
$$
\limsup\limits_{t\rightarrow0+} \frac{\lvert B(t) \rvert}{\sqrt{2t\ln\ln(1/t)}} = \limsup\limits_{t\rightarrow+\infty} \frac{t\lvert B(t^{-1}) \rvert}{\sqrt{2t\ln\ln(t)}} = \limsup\limits_{t\rightarrow+\infty} \frac{\lvert tB(t^{-1}) \rvert}{\sqrt{2t\ln\ln(t)}}
$$
<br/>According to part $(iii)$ of Theorem 2.1, we know that both $tB(t^{-1})$ and $-tB(t^{-1})$ are Brownian motions. Denote them as $B'(t)$ and $B''(t)$ respectively, we know that
$$
\frac{B''(t)}{\sqrt{2t\ln\ln(t)}} \leq \frac{\lvert tB(t^{-1}) \rvert}{\sqrt{2t\ln\ln(t)}} \leq \frac{B'(t)}{\sqrt{2t\ln\ln(t)}}.
$$
<br/> Take the limit superior of these equations as $t\rightarrow+\infty$, we can get
$$
\limsup\limits_{t\rightarrow0+} \frac{\lvert B(t) \rvert}{\sqrt{2t\ln\ln(1/t)}} = \limsup\limits_{t\rightarrow+\infty} \frac{\lvert tB(t^{-1}) \rvert}{\sqrt{2t\ln\ln(t)}} = 1 \quad a.s.
$$
<br/> using the law of iterated logarithm.


Q3

Denote $\tau:=\tau_{-a} \wedge \tau_{b}$, it's easy to show that $\tau$ is a stopping time. Since $B(t)$ is a martingale, we can know that
$$
\mathbb{E}(B(\tau)) = \mathbb{E}(B(0)) = 0.
$$
On the other hand, we have
$$
\mathbb{E}(B(\tau)) = -aP(B(\tau) = -a) + bP(B(\tau) = b) = -aP(\tau_{-a} < \tau_b) + b(1-P(\tau_{-a} < \tau_b)).
$$
So we can get that
$$
P(\tau_{-a} < \tau_b) = \frac{b}{a + b}.
$$
To calculate $\mathbb{E}(\tau_{-a} \wedge \tau_{b}) = \mathbb{E}(\tau)$, we construct the martingale $B^2(t) - t$. Since it's a martingale, we know that
$$
\mathbb{E}(B^2(\tau) - \tau) = \mathbb{E}(B^2(0) - 0) = 0.
$$
Also, we know that
$$
\mathbb{E}(B^2(\tau)) = a^2P(\tau_{-a} < \tau_b) + b^2(1-P(\tau_{-a} < \tau_b)) = ab.
$$
Then
$$
\mathbb{E}(\tau_{-a} \wedge \tau_{b}) = \mathbb{E}(\tau) = \mathbb{E}(B^2(\tau)) = ab
$$