{
 "cells": [
  {
   "cell_type": "markdown",
   "metadata": {},
   "source": [
    "## MTH9831 Assignment 2\n",
    "\n",
    "**Author: Boyu Yang, Julius Gruber, Yicheng Sun, Ziyuan Li**"
   ]
  },
  {
   "cell_type": "markdown",
   "metadata": {},
   "source": [
    "### Question 1"
   ]
  },
  {
   "cell_type": "markdown",
   "metadata": {},
   "source": [
    "From **Theorem 1.7**, we know that\n",
    "$$\n",
    "P(B^*(t) \\geq a, B(t) \\leq x) = 1 - N(\\frac{2a - x}{\\sqrt{t}})\n",
    "$$\n",
    "Then the cumulative distribution function of $(B(t), B^*(t))$ is\n",
    "$$\n",
    "\\begin{align*}\n",
    "F(a,x) &= P(B^*(t) \\leq a, B(t) \\leq x) = P(B(t)\\leq x) - P(B^*(t) \\geq a, B(t) \\leq x) \\\\\n",
    " &= \\int_{-\\infty}^x \\cfrac{1}{\\sqrt{2\\pi t}}e^{-\\frac{x^2}{2t}}dx - (1-N(\\cfrac{2a - x}{\\sqrt{t}}))\n",
    "\\end{align*}\n",
    "$$\n",
    "So the joint density of $(B(t), B^*(t))$ is \n",
    "$$\n",
    "f(x, a) = \\frac{\\partial^2 F}{\\partial x \\partial a} = \\cfrac{2(2a-x)}{t^{3/2}}\\phi(\\cfrac{2a-x}{\\sqrt{t}}),x\\leq a, a> 0\n",
    "$$\n",
    "where $\\phi(x)$ is the standard normal density function.\n"
   ]
  },
  {
   "cell_type": "markdown",
   "metadata": {},
   "source": [
    "### Question 2"
   ]
  },
  {
   "cell_type": "markdown",
   "metadata": {},
   "source": [
    "To start with\n",
    "$$\n",
    "\\limsup_{t\\to0^+} \\frac{|B(t)|}{\\sqrt{2t\\ln\\ln(1/t)}} = \\limsup_{s\\to+\\infty} \\frac{|B(s^{-1})|}{\\sqrt{(2/s)\\ln\\ln(s)}} = \\limsup_{s\\to+\\infty} \\frac{|sB(s^{-1})|}{\\sqrt{2s\\ln\\ln(s)}}\n",
    "$$\n",
    "\n",
    "According to part (iii) of Theorem 2.1, $B^*(t) = tB(t^{-1})$ is a Brownian motion. By using law of iterated logatithm\n",
    "$$\n",
    "\\limsup_{s\\to\\infty}\\frac{B(s)}{\\sqrt{2s\\ln\\ln(s)}} = 1 \\quad a.s.\n",
    "$$\n",
    "\n",
    "since we have\n",
    "$$\n",
    "|sB(s^{-1})| = max(B^*(s), -B^*(s))\n",
    "$$\n",
    "\n",
    "both of which are Brownian motion, so we can conclude that\n",
    "$$\n",
    "\\begin{align*}\n",
    "\\limsup_{s\\to+\\infty} \\frac{|sB(s^{-1})|}{\\sqrt{2s\\ln\\ln(s)}} &= \\limsup_{s\\to+\\infty} \\frac{max(B^*(s), -B^*(s))}{\\sqrt{2s\\ln\\ln(s)}} \\\\\n",
    "&= max(\\limsup_{s\\to\\infty}\\frac{B^*(s)}{\\sqrt{2s\\ln\\ln(s)}}, \\limsup_{s\\to\\infty}\\frac{-B^*(s)}{\\sqrt{2s\\ln\\ln(s)}}) \\\\\n",
    "&= 1 \\quad a.s\n",
    "\\end{align*}\n",
    "$$"
   ]
  },
  {
   "cell_type": "markdown",
   "metadata": {},
   "source": [
    "### Question 3"
   ]
  },
  {
   "cell_type": "markdown",
   "metadata": {},
   "source": [
    "(a) Denote $\\tau:=\\tau_{-a} \\wedge \\tau_{b}$, $\\tau$ is a stopping time since it adaptable to past information. Since $B(t)$ is a martingale, we can know that\n",
    "$$\n",
    "\\mathbb{E}(B(\\tau)) = \\mathbb{E}(B(0)) = 0\n",
    "$$\n",
    "$$\n",
    "\\mathbb{E}(B(\\tau)) = -aP(B(\\tau) = -a) + bP(B(\\tau) = b) = -aP(\\tau_{-a} < \\tau_b) + b(1-P(\\tau_{-a} < \\tau_b))\n",
    "$$\n",
    "$$\n",
    "\\Rightarrow P(\\tau_{-a} < \\tau_b) = \\frac{b}{a + b}\n",
    "$$\n",
    "\n",
    "(b) \n",
    "\n",
    "\n",
    "To calculate $\\mathbb{E}(\\tau_{-a} \\wedge \\tau_{b}) = \\mathbb{E}(\\tau)$, we construct the martingale $B^2(t) - t$. Since it's a martingale, we know that\n",
    "$$\n",
    "\\mathbb{E}(B^2(\\tau) - \\tau) = \\mathbb{E}(B^2(0) - 0) = 0.\n",
    "$$\n",
    "$$\n",
    "\\Rightarrow \\mathbb{E}(B^2(\\tau)) = a^2P(\\tau_{-a} < \\tau_b) + b^2(1-P(\\tau_{-a} < \\tau_b)) = ab.\n",
    "$$\n",
    "$$\n",
    "\\Rightarrow x\\mathbb{E}(\\tau_{-a} \\wedge \\tau_{b}) = \\mathbb{E}(\\tau) = \\mathbb{E}(B^2(\\tau)) = ab\n",
    "$$\n",
    "\t\t\t\t\t"
   ]
  },
  {
   "cell_type": "markdown",
   "metadata": {},
   "source": [
    "### Question 4"
   ]
  },
  {
   "cell_type": "markdown",
   "metadata": {},
   "source": [
    "### (i)\n",
    "1) $\\mathbb{E}[|Z(t)|] = mathbb{E}[Z(t)] = 1 < \\infty$ \n",
    "2) $Z(t)$ is $\\mathcal F$-measurable\n",
    "3) for $s\\le t$, we have\n",
    "$$\n",
    "\\begin{align*}\n",
    "\\mathbb{E}[Z(t)|\\mathcal F(s)] &= \\mathbb{E}[exp\\{\\sigma X(t) - (\\sigma\\mu + \\frac{1}{2}\\sigma^2)t\\}|\\mathcal F(s)] \\\\\n",
    "&= Z(s)\\mathbb{E}[exp\\{\\sigma(X(t)-X(s)) - (\\sigma\\mu + \\frac{1}{2}\\sigma^2)(t-s)\\}|\\mathcal F(s)] \\\\\n",
    "&= Z(s)\\mathbb{E}[exp\\{\\sigma(X(t)-X(s)) - (\\sigma\\mu + \\frac{1}{2}\\sigma^2)(t-s)\\}] \\\\\n",
    "&= Z(s)exp\\{-(\\sigma\\mu + \\frac{1}{2}\\sigma^2)(t-s)\\}\\mathbb{E}[exp\\{\\sigma(X(t)-X(s))\\}] \\\\\n",
    "&= Z(s)\n",
    "\\end{align*}\n",
    "$$\n",
    "\n",
    "Here we use the property: \n",
    "</br> (i) $X(t)-X(s)$ is independent with $\\mathcal F(s)$\n",
    "</br> (ii) $X(t)-X(s)$ ï½ž $N(\\mu t, \\sqrt{t-s})$\n",
    "\n",
    "so we can conclude $Z(t)$ is a martingale\n",
    "\n",
    "### (ii)\n",
    "$Z(t\\wedge\\tau_{m})$ is a stopped martingale. so we have\n",
    "$$\n",
    "1 = Z(0) = Z(t\\wedge\\tau_{m}) = \\mathbb{E}[exp\\{\\sigma X(t\\wedge\\tau_{m}) - (\\sigma\\mu + \\frac{1}{2}\\sigma^2)(t\\wedge\\tau_{m})\\}], \\quad t\\ge0\n",
    "$$\n",
    "\n",
    "### (iii)\n",
    "since we have \n",
    "$$\n",
    "0\\le exp\\{\\sigma X(t\\wedge\\tau_{m})\\}\\le e^{\\sigma m}\n",
    "$$\n",
    "which is bounded. take limit on both sides of the equation in (ii), we get\n",
    "$$\n",
    "\\lim_{t\\to\\infty}exp\\{\\sigma X(t\\wedge\\tau_{m}) - (\\sigma\\mu + \\frac{1}{2}\\sigma^2)(t\\wedge\\tau_{m})\\} = \\mathbb{I}_{(\\tau < \\infty)}exp\\{\\sigma m-(\\sigma\\mu + \\frac{1}{2}\\sigma^2)\\tau_{m}\\}\n",
    "$$\n",
    "so we have\n",
    "$$\n",
    "\\mathbb{E}[exp\\{\\sigma m-(\\sigma\\mu + \\frac{1}{2}\\sigma^2)\\tau_{m}\\}\\mathbb{I}_{(\\tau < \\infty)}] = 1 \\\\\n",
    "\\mathbb{E}[exp\\{-(\\sigma\\mu + \\frac{1}{2}\\sigma^2)\\tau_{m}\\}\\mathbb{I}_{(\\tau < \\infty)}] = e^{-\\sigma m}\n",
    "$$\n",
    "take limit on both sides as $\\sigma\\to 0$, we get $\\mathbb{E}[\\tau_m < \\infty] = 1$, equivalently\n",
    "$$\n",
    "\\mathbb{P}[\\tau_m < \\infty] = 1\n",
    "$$\n",
    "so we have\n",
    "$$\n",
    "\\mathbb{E}[exp\\{-(\\sigma\\mu + \\frac{1}{2}\\sigma^2)\\tau_{m}\\}] = e^{-\\sigma m}\n",
    "$$\n",
    "set $\\alpha = (\\sigma\\mu + \\frac{1}{2}\\sigma^2)$, since $\\sigma$ is positive, then we get $\\sigma = -\\mu + \\sqrt{2\\alpha + \\mu^2}$. \n",
    "</br> so for all $\\alpha > 0$, we have\n",
    "$$\n",
    "\\mathbb{E}[e^{-\\alpha\\tau_{m}}] = e^{m\\mu-m\\sqrt{2\\alpha + \\mu^2}}\n",
    "$$\n",
    "\n",
    "### (iv)\n",
    "take derivative with respect to $\\alpha$, then we have\n",
    "$$\n",
    "\\mathbb{E}[\\tau_m e^{-\\alpha\\tau_{m}}] = \\frac{m}{\\sqrt{2\\alpha+\\mu^2}}e^{m\\mu-m\\sqrt{2\\alpha + \\mu^2}}\n",
    "$$\n",
    "let $\\alpha\\to0$, we get \n",
    "$$\n",
    "\\mathbb{E}[\\tau_m] = \\frac{m}{\\mu}\n",
    "$$\n",
    "\n",
    "### (v)\n",
    "for $\\sigma > -2\\mu$, we have $\\sigma\\mu + \\frac{1}{2}\\sigma^2 > 0$. so similar as before, we have\n",
    "$$\n",
    "\\mathbb{E}[exp\\{\\sigma m-(\\sigma\\mu + \\frac{1}{2}\\sigma^2)\\tau_{m}\\}\\mathbb{I}_{(\\tau < \\infty)}] = 1 \\\\\n",
    "\\mathbb{E}[exp\\{-(\\sigma\\mu + \\frac{1}{2}\\sigma^2)\\tau_{m}\\}\\mathbb{I}_{(\\tau < \\infty)}] = e^{-\\sigma m}\n",
    "$$\n",
    "and then get\n",
    "\n",
    "\n",
    "\n",
    "1. Note that $W(t) \\sim \\mathcal{N}(0,t)$ and \n",
    "$$\n",
    "Z(t) = \\exp\\left\\{\\sigma W(t) - \\frac{1}{2}\\sigma^2t\\right\\},\n",
    "$$\n",
    "we can obtain that\n",
    "$$\n",
    "\\mathbb{E}|Z(t)| = \\int_{\\mathbb{R}}\\frac{1}{\\sqrt{2\\pi t}}e^{-\\frac{w^2}{2t}}\\cdot\\exp\\left\\{\\sigma w - \\frac{1}{2}\\sigma^2t\\right\\}dw=1<\\infty.\n",
    "$$\n",
    "2. $Z(t)$ is $\\mathcal{F}_t$-measurable because $Z(t)$ can be seen as a continuous function of $W(t)$ which is $\\mathcal{F}_t$-measurable by definition.\n",
    "3. For any $t\\geq s\\geq0$, we have\n",
    "$$\n",
    "\\begin{align*}\n",
    "\\mathbb{E}[Z(t)|W(s)] &= e^{\\sigma W(s)}\\mathbb{E}[\\exp\\left\\{\\sigma (W(t) - W(s))- \\frac{1}{2}\\sigma^2t\\right\\}|W(s)]\\\\\n",
    "&= e^{\\sigma W(s)}\\mathbb{E}[\\exp\\left\\{\\sigma (W(t) - W(s))- \\frac{1}{2}\\sigma^2t\\right\\}]\\\\\n",
    "&= e^{\\sigma W(s)}\\int_{\\mathbb{R}}\\frac{1}{\\sqrt{2\\pi (t-s)}}e^{-\\frac{w^2}{2(t-s)}}\\cdot\\exp\\left\\{\\sigma w - \\frac{1}{2}\\sigma^2t\\right\\}dw\\\\\n",
    "&= e^{\\sigma W(s)}\\exp\\left\\{\\frac{\\sigma^2}{2}(t-s) - \\frac{1}{2}\\sigma^2t\\right\\}dw\\\\\n",
    "&= \\exp\\left\\{\\sigma W(s) - \\frac{1}{2}\\sigma^2s\\right\\} = Z(s)\\\\\n",
    "\\end{align*}\n",
    "$$\n",
    "\n",
    "By 1-3, we conclude that W(t) is a martingale with respect to $\\mathcal{F}_t$.\n"
   ]
  }
 ],
 "metadata": {
  "language_info": {
   "name": "python"
  },
  "orig_nbformat": 4
 },
 "nbformat": 4,
 "nbformat_minor": 2
}
